Total.thy
@@ -3,7 +3,7 @@ imports "01Expression/Determinism" "02Stack/StackDeterminism" "02Stack/StackCorr
 begin
 
 theorem correct: "is_value e' \<Longrightarrow> revalue e' = (v, h) \<Longrightarrow> 
-    iter (op \<leadsto>) e e' = iter (op \<leadsto>\<^sub>s) (StackState (Eval e) [] empty\<^sub>h) (StackState (Return v) [] h)"
+    iter (op \<leadsto>) e e' = iter (op \<leadsto>\<^sub>s) (StackState (Eval e) [] empty\<^sub>h) (StackState (Return v) [] hh)"
   by simp
 
 end
